add hw2 base, hw1 final solutions

solutions/hw2/problem2.ml
@@ -1,0 +1,1 @@
+let compress : ('a -> 'a -> bool) -> 'a list -> 'a list
