solutions/hw1/isort.dfy
@@ -1,7 +1,16 @@
+ghost predicate Ordered(a: array<int>, left: nat, right: nat)
+  reads a
+  requires left <= right <= a.Length
+{
+  forall i: nat :: 0 < left <= i < right ==> a[i-1] <= a[i]
+}
+
 method SelectionSort(a: array<int>)
   modifies a
+  ensures Ordered(a, 0, a.Length)
 {
   for i := 0 to a.Length
+    // invariant Ordered(a, 0, i)
   {
     var minValue := a[i];
     var minPos := i;
